adding forall and map to dependent monotonic map

ulib/FStar.Monotonic.DependentMap.fsti
@@ -210,3 +210,26 @@ val lookup
             contains t x v h1 /\
             MR.witnessed (contains t x v))))
  
+let forall_t (#a:eqtype) (#b:a -> Type) (#inv:DM.t a (opt b) -> Type) (#r:MR.rid)
+             (t:t r a b inv) (h:HS.mem) (pred: (x:a) -> b x -> Type0)
+  = forall (x:a).{:pattern (sel (MR.m_sel h t) x) \/ (DM.sel (repr (MR.m_sel h t)) x)}
+            defined t x h ==> pred x (Some?.v (sel (MR.m_sel h t) x))
+
+let f_opt (#a:eqtype) (#b #c:a -> Type) (f: (x:a) -> b x -> c x) :(x:a) -> option (b x) -> option (c x)
+  = fun x y ->
+    match y with
+    | None   -> None
+    | Some y -> Some (f x y)
+
+val mmap_f (#a:eqtype) (#b #c:a -> Type) (m:map a b) (f: (x:a) -> b x -> c x)
+  :Tot (m':(map a c){repr m' == DM.map (f_opt f) (repr m)})
+
+val map_f (#a:eqtype) (#b #c:a -> Type)
+          (#inv:DM.t a (opt b) -> Type) (#inv':DM.t a (opt c) -> Type)
+	  (#r #r':MR.rid)
+          (m:t r a b inv) (f: (x:a) -> b x -> c x)
+	  :ST (t r' a c inv')
+	      (requires (fun h0 -> inv' (DM.map (f_opt f) (repr (MR.m_sel h0 m)))))
+	      (ensures  (fun h0 m' h1 ->
+	                 inv' (DM.map (f_opt f) (repr (MR.m_sel h0 m))) /\  //AR: surprised that even after the fix for #57, we need this repetetion from the requires clause
+	                 ralloc_post r' (mmap_f (MR.m_sel h0 m) f) h0 (MR.as_hsref m') h1))
